\chapter{Slater-Koster hoppings}
\label{SKhoppings}
In this chapter we just summarize the \ac{sk} hoppings. In every case it is assumed that the orbitals are separated by a vector $\vec{r}$ and

\begin{equation*}
  \vec{r} \longrightarrow \hat{r}=\frac{\vec{r}}{|\vec{r}|} = (l,m,n)
\end{equation*}

The formulas for the $s-p$ hoppings are:
\begin{equation}
\begin{split}
  t_{ss} &= V_{ss\sigma}\\
  t_{sp_x} &= l V_{ss\sigma}\\
\end{split}
\end{equation}
by symmetry it follows that:
\begin{equation}
   t_{sp_y}(l,m,n) = t_{sp_x}(m,-l,n) \qquad \text{and} \qquad
   t_{sp_z}(l,m,n) = t_{sp_x}(n,m,-l)
\end{equation}
The formulas for hoppings among the $p$ orbitals are:
\begin{equation}
\begin{split}
  t_{p_x-p_x} &= l^2 V_{pp\sigma} + \left(1-l^2\right) V_{pp\pi}\\
  t_{p_x-p_y} &= lm V_{pp\sigma} - lm V_{pp\pi}\\
  t_{p_x-p_z} &= ln V_{pp\sigma} - ln V_{pp\pi}
\end{split}
\end{equation}
which imply that:
\begin{equation}
\begin{split}
   t_{p_yp_y}(l,m,n) &= t_{p_xp_x}(m,-l,n) \\
   t_{p_yp_z}(l,m,n) &= t_{p_xp_y}(m,n,l) \\
   t_{p_zp_z}(l,m,n) &= t_{p_zp_z}(n,m,-l)
\end{split}
\end{equation}

the formulas for the $s-d$ hoppings are:
\begin{equation*}
\begin{split}
  t_{s-d_{xy}} &= \sqrt{3}lm V_{sd\sigma}\\
  t_{s-d_{x^2-y^2}} &= \tfrac{\sqrt{3}}{2} (l^2-m^2) V_{sd\sigma}\\
  t_{s-d_{3x^2-r^2}} &= \left[n^2-\frac{1}{2}(l^2+m^2)\right] V_{sd\sigma}
\end{split}
\end{equation*}
for the $p-d$ hoppings:
\begin{equation*}
\begin{split}
  t_{p_x-d_{xy}} &= \sqrt{3}l^2m V_{pd\sigma} + m(1-2l^2) V_{pd\pi}\\
  t_{p_x-d_{yz}} &= \sqrt{3}lmn V_{pd\sigma} - 2lmn V_{pd\pi}\\
  t_{p_x-d_{zx}} &= \sqrt{3}l^2n V_{pd\sigma} + n(1-2l^2) V_{pd\pi}\\
  t_{p_x-d_{x^2-y^2}} &= \frac{\sqrt{3}}{2}l(l^2-m^2) V_{pd\sigma} +
                         l(1-l^2+m^2) V_{pd\pi}\\
  t_{p_y-d_{x^2-y^2}} &= \tfrac{\sqrt{3}}{2}m(l^2-m^2) V_{pd\sigma} -
                         m(1+l^2-m^2) V_{pd\pi}\\
  t_{p_z-d_{x^2-y^2}} &= \tfrac{\sqrt{3}}{2}n(l^2-m^2) V_{pd\sigma} -
                         n(l^2-m^2) V_{pd\pi}\\
  t_{p_x-d_{3z^2-r^2}} &= l\left[n^2-\tfrac{1}{2}(l^2+m^2)\right] V_{pd\sigma}-
                          \sqrt{3}ln^2 V_{pd\pi}\\
  t_{p_y-d_{3z^2-r^2}} &= m\left[n^2-\tfrac{1}{2}(l^2+m^2)\right] V_{pd\sigma}-
                          \sqrt{3}mn^2 V_{pd\pi}\\
  t_{p_z-d_{3z^2-r^2}} &= n\left[n^2-\tfrac{1}{2}(l^2+m^2)\right] V_{pd\sigma}+
                          \sqrt{3}n(l^2+m^2) V_{pd\pi}
\end{split}
\end{equation*}
and inter-$d$ hoppings:
\begin{equation*}
\begin{split}
  t_{d_{xy}-d_{xy}} &= 3l^2m^2 V_{dd\sigma} + (l^2 + m^2 - 4l^2m^2) V_{dd\pi}+
                       (n^2+l^2m^2) V_{dd\delta}\\
  t_{d_{xy}-d_{yz}} &= 3lm^2n V_{dd\sigma} + ln(1-4m^2) V_{dd\pi}+
                       ln(m^2-1) V_{dd\delta}\\
  t_{d_{xy}-d_{zx}} &= 3l^2mn V_{dd\sigma} + mn(1-4l^2) V_{dd\pi}+
                       mn(l^2-1) V_{dd\delta}\\
  t_{d_{xy}-d_{x^2-y^2}} &= \tfrac{3}{2}lm(l^2-m^2) V_{dd\sigma} +
                            2lm(m^2-l^2) V_{dd\pi}+
                            \tfrac{1}{2}lm(l^2-m^2) V_{dd\delta}\\
  t_{d_{yz}-d_{x^2-y^2}} &= \tfrac{3}{2}mn(l^2-m^2) V_{dd\sigma} -
                            mn\left[1+2(l^2-m^2)\right]V_{dd\pi}+
                            mn\left[1+\tfrac{1}{2}(l^2-m^2)\right] V_{dd\delta}
\end{split}  % TODO some are still missing
\end{equation*}


\newpage
\begin{table}
\centering
\begin{tabular}{|r|l|}
 \hline
 Hopping & Slater-Koster formula \\ \hline
 $s-s=$ & $V_{ss\sigma}$ \\ \hline\hline
 $s-p_x=$ & $lV_{ss\sigma}$\\ \hline
 $s-p_y=$ & $t_{sp_x}(m,-l,n)$\\ \hline
 $s-p_z=$ & $t_{sp_x}(n,m,-l)$\\ \hline\hline
 
 $p_x-p_x=$ & $l^2 V_{pp\sigma} + \left(1-l^2\right) V_{pp\pi}$\\ \hline
 $p_x-p_y=$ & $lm V_{pp\sigma} - lm V_{pp\pi}$\\ \hline
 $p_x-p_z=$ & $ln V_{pp\sigma} - ln V_{pp\pi}$\\ \hline
 $p_y-p_y=$ & $t_{p_xp_x}(m,-l,n)$ \\ \hline
 $p_y-p_z=$ & $t_{p_xp_y}(m,n,l)$ \\ \hline
 $p_z-p_z=$ & $t_{p_zp_z}(n,m,-l)$ \\ \hline\hline
 
 $s-d_{xy}=$ & $\sqrt{3}lm V_{sd\sigma}$\\ \hline
 $s-d_{yz}=$ & $t_{sd_{xy}}(n,m,-l)$\\ \hline
 $s-d_{zx}=$ & $t_{sd_{xy}}(l,n,-m)$\\ \hline
 $s-d_{x^2-y^2}=$ & $\tfrac{\sqrt{3}}{2} (l^2-m^2) V_{sd\sigma}$\\ \hline
 $s-d_{3x^2-r^2}=$ & $ \left[n^2-\frac{1}{2}(l^2+m^2)\right] V_{sd\sigma}$\\ \hline\hline
 $p_x-d_{xy}=$ & $\sqrt{3}l^2m V_{pd\sigma} + m(1-2l^2) V_{pd\pi}$\\ \hline
 $p_x-d_{yz}=$ & $\sqrt{3}lmn V_{pd\sigma} - 2lmn V_{pd\pi}$\\ \hline
 $p_x-d_{zx}=$ & $\sqrt{3}l^2n V_{pd\sigma} + n(1-2l^2) V_{pd\pi}$\\ \hline
 $p_x-d_{x^2-y^2}=$ & $\frac{\sqrt{3}}{2}l(l^2-m^2) V_{pd\sigma} + l(1-l^2+m^2) V_{pd\pi}$\\ \hline
 $p_y-d_{x^2-y^2}=$ & $\tfrac{\sqrt{3}}{2}m(l^2-m^2) V_{pd\sigma} - m(1+l^2-m^2) V_{pd\pi}$\\ \hline
 $p_z-d_{x^2-y^2}=$ & $\tfrac{\sqrt{3}}{2}n(l^2-m^2) V_{pd\sigma} - n(l^2-m^2) V_{pd\pi}$\\ \hline
 $p_x-d_{3z^2-r^2}=$ & $l\left[n^2-\tfrac{1}{2}(l^2+m^2)\right] V_{pd\sigma}-\sqrt{3}ln^2 V_{pd\pi}$\\ \hline
 $p_y-d_{3z^2-r^2}=$ & $m\left[n^2-\tfrac{1}{2}(l^2+m^2)\right] V_{pd\sigma}-\sqrt{3}mn^2 V_{pd\pi}$\\ \hline
 $p_z-d_{3z^2-r^2}=$ & $n\left[n^2-\tfrac{1}{2}(l^2+m^2)\right] V_{pd\sigma}+ \sqrt{3}n(l^2+m^2) V_{pd\pi}$\\ \hline\hline
 
 $d_{xy}-d_{xy}=$ & $3l^2m^2 V_{dd\sigma} + (l^2 + m^2 - 4l^2m^2) V_{dd\pi}+ (n^2+l^2m^2) V_{dd\delta}$\\ \hline
 $d_{xy}-d_{yz}=$ & $3lm^2n V_{dd\sigma} + ln(1-4m^2) V_{dd\pi}+ ln(m^2-1) V_{dd\delta}$\\ \hline
 $d_{xy}-d_{zx}=$ & $3l^2mn V_{dd\sigma} + mn(1-4l^2) V_{dd\pi}+ mn(l^2-1) V_{dd\delta}$\\ \hline
 $d_{xy}-d_{x^2-y^2}=$ & $\tfrac{3}{2}lm(l^2-m^2) V_{dd\sigma} + 2lm(m^2-l^2) V_{dd\pi}+ \tfrac{1}{2}lm(l^2-m^2) V_{dd\delta}$\\ \hline
 $d_{yz}-d_{x^2-y^2}=$ & $\tfrac{3}{2}mn(l^2-m^2) V_{dd\sigma} - mn\left[1+2(l^2-m^2)\right]V_{dd\pi}+ mn\left[1+\tfrac{1}{2}(l^2-m^2)\right] V_{dd\delta}$\\ \hline
\end{tabular}
\end{table}
